src/Common/OptionFacts.v
@@ -1,5 +1,21 @@
+Require Import Coq.Classes.Morphisms.
+
 Lemma option_map_None A B (f : A -> B) x
 : option_map f x = None <-> x = None.
 Proof.
   destruct x; simpl; split; intros; trivial; congruence.
+Qed.
+
+Global Instance option_rect_Proper_nondep {A B}
+: Proper (pointwise_relation _ eq ==> eq ==> eq ==> eq)
+         (@option_rect A (fun _ => B)).
+Proof.
+  repeat (intros [] || intro); simpl; eauto.
+Qed.
+
+Global Instance option_rect_Proper {A B}
+: Proper (forall_relation (fun _ => eq) ==> eq ==> forall_relation (fun _ => eq))
+         (@option_rect A B).
+Proof.
+  repeat (intros [] || intro); simpl; eauto.
 Qed.
